all_different added, n_value partially done

examples/pseudo_bool/cp_encoding/cp_to_ilp_countingScript.sml
@@ -9,7 +9,7 @@ Ancestors
 
 Definition neiv_def[simp]:
   neiv name (i:num) j =
-    INR (name, Indices [i;j] (SOME $ strlit "ne"))
+    INR (name, Indices [i;j] NONE)
 End
 
 (* AllDifferent: All variables must take distinct values
@@ -34,12 +34,35 @@ Theorem encode_all_different_sem_1:
     (encode_all_different bnd Xs name)
 Proof
   rw[encode_all_different_def,all_different_sem_def,EVERY_MEM]>>
-  gs[MEM_FLAT,indexedListsTheory.MEM_MAPi]>>
+  gs[MEM_FLAT,MEM_MAPi]>>
   Cases_on ‘i < j’>>
   gs[reify_avar_def,reify_flag_def]
   >- intLib.ARITH_TAC>>
-  gvs[EL_ALL_DISTINCT_EL_EQ]>>
-  cheat
+  rw[]>>
+  fs[EL_ALL_DISTINCT_EL_EQ,EL_MAP]>>
+  first_x_assum $ qspecl_then [‘i’,‘j’] assume_tac>>
+  intLib.ARITH_TAC
+QED
+
+Theorem all_different_sem_aux:
+  (∀i j. i < j ∧ j < LENGTH Xs ⇒
+    let X = EL i Xs in
+    let Y = EL j Xs in
+    if wb (neiv name i j)
+    then varc wi X > varc wi Y
+    else varc wi Y > varc wi X) ⇒
+  all_different_sem Xs wi
+Proof
+  rw[all_different_sem_def,EL_ALL_DISTINCT_EL_EQ]>>
+  Cases_on`n1 = n2`>>simp[]>>
+  wlog_tac `n1 < n2` [`n1`,`n2`]
+  >- (
+    `n2 < n1` by fs[]>>
+    first_x_assum drule_all>>
+    simp[])>>
+  first_x_assum drule>>
+  rw[EL_MAP]>>
+  intLib.ARITH_TAC
 QED
 
 Theorem encode_all_different_sem_2:
@@ -48,16 +71,315 @@ Theorem encode_all_different_sem_2:
     (encode_all_different bnd Xs name) ⇒
   all_different_sem Xs wi
 Proof
-  cheat
+  strip_tac>>
+  irule all_different_sem_aux>>
+  gs[EVERY_MEM,encode_all_different_def,MEM_FLAT,MEM_MAPi,PULL_EXISTS]>>
+  qexistsl [‘name’,‘wb’]>>
+  ntac 3 strip_tac>>
+  ‘i < LENGTH Xs’ by fs[]>>
+  first_x_assum $ drule_then rev_drule>>
+  simp[SF DNF_ss]>>
+  rw[]>>
+  intLib.ARITH_TAC
+QED
+
+(* domain of X given by bnd (as a list) *)
+Definition domlist_def:
+  domlist bnd (X:'a varc) =
+  case X of
+    INL vX =>
+      (let
+        (lb, ub) = bnd vX
+      in
+        if ub < lb
+        then []
+        else GENLIST (λn. &n + lb) (Num (ub - lb) + 1))
+  | INR cX => [cX]
+End
+
+Theorem MEM_domlist:
+  valid_assignment bnd wi ⇒
+  MEM (varc wi X) (domlist bnd X)
+Proof
+  Cases_on ‘X’>>
+  rw[domlist_def,valid_assignment_def,varc_def]>>
+  rename1 ‘bnd x’>>
+  Cases_on ‘bnd x’>>
+  rw[MEM_GENLIST]>>
+  res_tac
+  >-intLib.ARITH_TAC>>
+  qexists ‘Num (wi x - q)’>>
+  intLib.ARITH_TAC
+QED
+
+(* bijection 0, -1, 1, -2, 2,... ⇔ 0, 1, 2, 3, 4,... and its inverse next *)
+Definition intnum_def:
+  intnum (n: int) =
+  if n < 0 then 2 * Num (-n) - 1
+  else 2 * Num n
+End
+
+Definition numint_def:
+  numint (n: num): int =
+  if EVEN n then &((n + 1) DIV 2)
+  else -&((n + 1) DIV 2)
+End
+
+Theorem numint_inj:
+  numint m = numint n ⇒ m = n
+Proof
+  simp[numint_def]>>
+  intLib.ARITH_TAC
+QED
+
+Theorem numint_intnum:
+  numint (intnum x) = x
+Proof
+  simp[intnum_def,numint_def]>>
+  intLib.ARITH_TAC
+QED
+
+Theorem intnum_numint:
+  intnum (numint x) = x
+Proof
+  simp[intnum_def,numint_def]>>
+  intLib.ARITH_TAC
+QED
+
+Definition numset_to_intlist_def:
+  numset_to_intlist t = MAP (numint o FST) $ toSortedAList t
+End
+
+Theorem ALL_DISTINCT_numset_to_intlist:
+  ALL_DISTINCT $ numset_to_intlist t
+Proof
+  simp[numset_to_intlist_def,GSYM MAP_MAP_o]>>
+  irule ALL_DISTINCT_MAP_INJ>>
+  simp[ALL_DISTINCT_MAP_FST_toSortedAList,numint_inj]
+QED
+
+(* Union of all int values in domains of Xs *)
+Definition union_dom_def:
+  union_dom bnd Xs =
+  numset_to_intlist $ FOLDL union LN $
+    MAP (λX. list_to_num_set $ MAP intnum $ domlist bnd X) Xs
+End
+
+Theorem MEM_numset_to_intlist:
+  MEM x (numset_to_intlist ns) ⇔
+  intnum x ∈ domain ns
+Proof
+  rw[numset_to_intlist_def,GSYM MAP_MAP_o,MEM_MAP,EXISTS_PROD,
+    MEM_toSortedAList,domain_lookup]>>
+  metis_tac[intnum_numint,numint_intnum]
+QED
+
+Theorem domain_FOLDL_union:
+  ∀ls t.
+  x ∈ domain (FOLDL union t ls) ⇔
+  x ∈ domain t ∨ ∃ns. ns ∈ set ls ∧ x ∈ domain ns
+Proof
+  Induct>>rw[]>>
+  metis_tac[]
+QED
+
+Theorem EVERY_MEM_union_dom:
+  valid_assignment bnd wi ⇒
+  EVERY (λX. MEM (varc wi X) (union_dom bnd Xs)) Xs
+Proof
+  rw[EVERY_MEM,union_dom_def,MEM_numset_to_intlist,domain_FOLDL_union]>>
+  simp[MEM_MAP,PULL_EXISTS,domain_list_to_num_set]>>
+  metis_tac[MEM_domlist]
+QED
+
+Theorem ALL_DISTINCT_union_dom:
+  ALL_DISTINCT $ union_dom bnd Xs
+Proof
+  simp[union_dom_def,ALL_DISTINCT_numset_to_intlist]
+QED
+
+Definition elm_def[simp]:
+  elm name (v:int) =
+  INR (name, Values [v] NONE)
+End
+
+(* encodes fnvalue_v ⇔ some X = v *)
+Definition encode_some_eq_def:
+  encode_some_eq bnd Xs (v: int) name =
+    bimply_bits bnd [Pos (elm name v)]
+      ([], MAP (λX. (1i, Pos (INL (Eq X v)))) Xs, 1i)
+End
+
+Theorem iSUM_ge_0:
+  (∀x. MEM x ls ⇒ x ≥ 0) ⇒
+  iSUM ls ≥ 0
+Proof
+  Induct_on`ls`>> rw[iSUM_def]>>
+  fs[SF DNF_ss]>>
+  intLib.ARITH_TAC
+QED
+
+Theorem b2i_alt:
+  b2i b = if b then 1 else 0
+Proof
+  rw[]
+QED
+
+Theorem eval_lin_term_ge_1:
+  eval_lin_term wb (MAP (λe. (1, f e)) ls) ≥ 1 ⇔
+  ∃e. MEM e ls ∧ lit wb (f e)
+Proof
+  rw[eval_lin_term_def]>>
+  Induct_on ‘ls’>>
+  rw[iSUM_def,b2i_alt]
+  >-(
+    simp[SF DNF_ss]>>
+    qmatch_goalsub_abbrev_tac`_ + iSUM lss ≥ _`>>
+    `iSUM lss ≥ 0` by (
+      irule iSUM_ge_0>>
+      simp[Abbr`lss`,MEM_MAP,PULL_EXISTS,b2i_alt]>>
+      rw[])>>
+    intLib.ARITH_TAC)
+  >- metis_tac[]
+QED
+
+Theorem encode_some_eq_sem:
+  valid_assignment bnd wi ∧
+  EVERY (λX. wb (INL (Eq X v)) ⇔ varc wi X = v) Xs ⇒
+  (EVERY (λx. iconstraint_sem x (wi,wb)) (encode_some_eq bnd Xs v name) =
+  (wb (elm name v) ⇔ ∃X. MEM X Xs ∧ wb (INL (Eq X v))))
+Proof
+  rw[encode_some_eq_def,iconstraint_sem_def,eval_lin_term_ge_1]>>
+  metis_tac[]
+QED
+
+Definition reify_some_eq_def:
+  reify_some_eq bnd Xs v name =
+  let
+    ges = FLAT $ MAP (λX. encode_ge bnd X v ++ encode_ge bnd X (v + 1)) Xs;
+    eqs = FLAT $ MAP (λX. encode_eq bnd X v) Xs
+  in
+    ges ++ eqs ++ encode_some_eq bnd Xs v name
+End
+
+Theorem FORALL_IMP_EQ[local] = METIS_PROVE []
+  ``(∀x. P x ⇒ (Q x ⇔ R x)) ⇒ ((∀x. P x ⇒ Q x) ⇔ (∀x. P x ⇒ R x))``;
+
+Theorem reify_some_eq_sem:
+  valid_assignment bnd wi ⇒ (
+  EVERY (λx. iconstraint_sem x (wi,wb)) (FLAT (MAP (λv. reify_some_eq bnd Xs v name)
+    (union_dom bnd Xs))) ⇔
+  ∀v. MEM v (union_dom bnd Xs) ⇒
+      EVERY (λX. wb (INL (Ge X v)) ⇔ varc wi X ≥ v) Xs ∧
+      EVERY (λX. wb (INL (Ge X (v + 1))) ⇔ varc wi X ≥ v + 1) Xs ∧
+      EVERY (λX. wb (INL (Eq X v)) ⇔ varc wi X = v) Xs ∧
+      (wb (elm name v) ⇔ ∃X. MEM X Xs ∧ wb (INL (Eq X v))))
+Proof
+  rw[reify_some_eq_def,EVERY_FLAT,EVERY_MAP]>>
+  simp[Once EVERY_MEM,Once $ GSYM CONJ_ASSOC]>>
+  ho_match_mp_tac FORALL_IMP_EQ>>
+  rw[EVERY_CONJ,GSYM CONJ_ASSOC]>>
+  match_mp_tac LEFT_AND_CONG>>
+  CONJ_TAC
+  >- (irule EVERY_CONG>>simp[encode_ge_sem])>>
+  strip_tac>>
+  match_mp_tac LEFT_AND_CONG>>
+  CONJ_TAC
+  >- (irule EVERY_CONG>>simp[encode_ge_sem])>>
+  strip_tac>>
+  match_mp_tac LEFT_AND_CONG>>
+  CONJ_TAC
+  >- (
+    irule EVERY_CONG>>
+    rw[]>>
+    irule encode_eq_sem>>
+    fs[EVERY_MEM])>>
+  simp[encode_some_eq_sem]
+QED
+
+(* encodes (sum of the bitlist Bs) = Y *)
+Definition encode_bitsum_def:
+  encode_bitsum Bs Y =
+  case Y of
+    INL vY => [
+      ([(-1i, vY)], MAP (λb. (1i, Pos b)) Bs, 0i);
+      ([(1i, vY)], MAP (λb. (-1i, Pos b)) Bs, 0i)]
+  | INR cY => [
+      ([], MAP (λb. (1i, Pos b)) Bs, cY);
+      ([], MAP (λb. (-1i, Pos b)) Bs, -cY)]
+End
+
+Theorem iSUM_MAP_lin:
+  ∀ls a f b. iSUM (MAP (λx. a * f x + b) ls) = a * iSUM (MAP (λx. f x) ls) + b * &LENGTH ls
+Proof
+  Induct>>
+  simp[iSUM_def,MAP,LENGTH]>>
+  rw[]>>
+  intLib.ARITH_TAC
+QED
+
+Theorem iSUM_MAP_lin_const = iSUM_MAP_lin |> CONV_RULE (RESORT_FORALL_CONV List.rev) |> Q.SPEC `0` |> SRULE [] |> SPEC_ALL;
+
+Theorem encode_bitsum_sem:
+  valid_assignment bnd wi ⇒
+  (EVERY (λx. iconstraint_sem x (wi,wb)) (encode_bitsum Bs Y) ⇔
+  iSUM $ MAP (b2i o wb) Bs = varc wi Y)
+Proof
+  rw[encode_bitsum_def]>>
+  CASE_TAC>>
+  simp[varc_def,iconstraint_sem_def,eval_ilin_term_def,eval_lin_term_def,
+    eval_iterm_def,eval_term_def,iSUM_def,MAP_MAP_o,combinTheory.o_ABS_R,
+    iSUM_MAP_lin_const]>>
+  simp[GSYM combinTheory.o_ABS_R,GSYM combinTheory.I_EQ_IDABS]>>
+  intLib.ARITH_TAC
+QED
+
+Theorem encode_nvalue_sem_aux:
+  valid_assignment bnd wi ∧
+  (∀v. MEM v (union_dom bnd Xs) ⇒
+    EVERY (λX. wb (INL (Eq X v)) ⇔ varc wi X = v) Xs ∧
+    (wb (elm name v) ⇔ ∃X. MEM X Xs ∧ wb (INL (Eq X v)))) ⇒
+  ∀v. MEM v (MAP (varc wi) Xs) ⇔ MEM v (FILTER (λv. wb (elm name v)) (union_dom bnd Xs))
+Proof
+  rw[MEM_FILTER,MEM_MAP]>>
+  iff_tac>>
+  strip_tac
+  >-(
+    CONJ_ASM2_TAC
+    >- (
+      gvs[EVERY_MEM]>>
+      metis_tac[])>>
+    drule_then assume_tac EVERY_MEM_union_dom>>
+    fs[EVERY_MEM])>>
+  gvs[EVERY_MEM]>>
+  metis_tac[]
+QED
+
+Theorem list_set_eq:
+  ∀ls1 ls2. (∀v. MEM v ls1 ⇔ MEM v ls2) ⇔ set ls1 = set ls2
+Proof
+  rw[SET_EQ_SUBSET]>>
+  simp[GSYM SUBSET_DIFF_EMPTY,list_to_set_diff,GSYM NULL_EQ,NULL_FILTER]>>
+  metis_tac[]
+QED
+
+Theorem iSUM_FILTER:
+  iSUM (MAP (b2i o P) ls) = &(LENGTH $ FILTER P ls)
+Proof
+  Induct_on ‘ls’>>
+  rw[iSUM_def]>>
+  intLib.ARITH_TAC
 QED
 
 (* NValue: Y equals the number of distinct values in Xs
    This is very complex and requires auxiliary variables *)
 Definition encode_n_value_def:
-  encode_n_value bnd Xs Y =
-  (* TODO: Complex encoding requiring auxiliary variables
-     for each potential value in the domain *)
-  [false_constr]
+  encode_n_value bnd Xs Y name =
+  let
+    vals = union_dom bnd Xs
+  in
+    (FLAT $ MAP (λv. reify_some_eq bnd Xs v name) vals) ++
+    encode_bitsum (MAP (elm name) vals) Y
 End
 
 Theorem encode_n_value_sem_1:
